src/compiler/meta/OCL_compiler_meta_META.thy
@@ -160,24 +160,40 @@ datatype hol_thy_extended = (* pure Isabelle *)
 
 subsection{* ... *}
 
-definition "Thy_dataty = Isab_thy o Theory_dataty"
-definition "Thy_ty_synonym = Isab_thy o Theory_ty_synonym"
-definition "Thy_ty_notation = Isab_thy o Theory_ty_notation"
-definition "Thy_instantiation_class = Isab_thy o Theory_instantiation_class"
-definition "Thy_defs_overloaded = Isab_thy o Theory_defs_overloaded"
-definition "Thy_consts_class = Isab_thy o Theory_consts_class"
-definition "Thy_definition_hol = Isab_thy o Theory_definition_hol"
-definition "Thy_lemmas_simp = Isab_thy o Theory_lemmas_simp"
-definition "Thy_lemma_by = Isab_thy o Theory_lemma_by"
-definition "Thy_axiom = Isab_thy o Theory_axiom"
-definition "Thy_section_title = Isab_thy o Theory_section_title"
-definition "Thy_text = Isab_thy o Theory_text"
-definition "Thy_ml = Isab_thy o Theory_ml"
-definition "Thy_thm = Isab_thy o Theory_thm"
+definition "Thy_dataty = Isab_thy o H_thy_simple o Theory_dataty"
+definition "Thy_ty_synonym = Isab_thy o H_thy_simple o Theory_ty_synonym"
+definition "Thy_ty_notation = Isab_thy o H_thy_simple o Theory_ty_notation"
+definition "Thy_instantiation_class = Isab_thy o H_thy_simple o Theory_instantiation_class"
+definition "Thy_defs_overloaded = Isab_thy o H_thy_simple o Theory_defs_overloaded"
+definition "Thy_consts_class = Isab_thy o H_thy_simple o Theory_consts_class"
+definition "Thy_definition_hol = Isab_thy o H_thy_simple o Theory_definition_hol"
+definition "Thy_lemmas_simp = Isab_thy o H_thy_simple o Theory_lemmas_simp"
+definition "Thy_lemma_by = Isab_thy o H_thy_simple o Theory_lemma_by"
+definition "Thy_axiom = Isab_thy o H_thy_simple o Theory_axiom"
+definition "Thy_section_title = Isab_thy o H_thy_simple o Theory_section_title"
+definition "Thy_text = Isab_thy o H_thy_simple o Theory_text"
+definition "Thy_ml = Isab_thy o H_thy_simple o Theory_ml"
+definition "Thy_thm = Isab_thy o H_thy_simple o Theory_thm"
+
+definition "Thy_dataty' = Theory_dataty"
+definition "Thy_ty_synonym' = Theory_ty_synonym"
+definition "Thy_ty_notation' = Theory_ty_notation"
+definition "Thy_instantiation_class' = Theory_instantiation_class"
+definition "Thy_defs_overloaded' = Theory_defs_overloaded"
+definition "Thy_consts_class' = Theory_consts_class"
+definition "Thy_definition_hol' = Theory_definition_hol"
+definition "Thy_lemmas_simp' = Theory_lemmas_simp"
+definition "Thy_lemma_by' = Theory_lemma_by"
+definition "Thy_axiom' = Theory_axiom"
+definition "Thy_section_title' = Theory_section_title"
+definition "Thy_text' = Theory_text"
+definition "Thy_ml' = Theory_ml"
+definition "Thy_thm' = Theory_thm"
 
 subsection{* ... *}
 
-definition "hol_map_thy f = (\<lambda> Isab_thy x \<Rightarrow> Isab_thy (f x)
+definition "hol_map_thy f = (\<lambda> Isab_thy (H_thy_simple x) \<Rightarrow> Isab_thy (H_thy_simple (f x))
+                             | Isab_thy (H_thy_locale data l) \<Rightarrow> Isab_thy (H_thy_locale data (List_map (List_map f) l))
                              | x \<Rightarrow> x)"
 
 end
